

# MAT315 - Homework 1 / Homework 3

Sean Andrade

February 2026

## 3B

7. Pick a basis  $\{v_1, v_2, \dots, v_n\}$  of  $V$  and  $\{w_1, w_2, \dots, w_n, \dots, w_m\}$  of  $W$ . ( $\dim V \leq \dim W$ )

$V$  has dimension at least two. So define the following two maps on  $V$ :

$$\begin{aligned} f_1 \left( \sum_{i=1}^n a_i v_i \right) &= a_n w_n + \frac{1}{2} \sum_{i=2}^{n-1} a_i w_i \\ f_2 \left( \sum_{i=1}^n a_i v_i \right) &= a_1 w_1 + \frac{1}{2} \sum_{i=2}^{n-1} a_i w_i \end{aligned}$$

Again,  $n = \dim V \geq 2$  and so these sums on the right are not empty sums. Also,  $v_1$  is distinct from  $v_n$ .

These maps are well-defined because the representation of a vector as a linear combination of basis elements is unique. They are easily checked to be linear; this is done by the proof of Axler 3.4.

Neither of these maps are injective, because the nonzero vector  $v_1$  gets sent to zero by  $f_1$  and the nonzero vector  $v_n$  gets sent to zero by  $f_2$  (basis vectors are nonzero).

However, their sum is the map:

$$(f_1 + f_2) \left( \sum_{i=1}^n a_i v_i \right) = a_1 w_1 + \frac{1}{2} \sum_{i=2}^{n-1} a_i w_i + \frac{1}{2} \sum_{i=2}^{n-1} a_i w_i + a_n w_n = \sum_{i=1}^n a_i w_i$$

and this map is injective, because a vector  $\sum_{i=1}^n a_i v_i$  goes to zero under this map if and only if  $\sum_{i=1}^n a_i w_i = 0$  (by definition). But since the vectors  $\{w_1, \dots, w_n\}$  are linearly independent (as a subset of the basis vectors), this only happens if  $a_i = 0$  for all  $i$ , which happens if and only if the input vector  $\sum_{i=1}^n a_i v_i = 0$ . Thus  $\ker(f_1 + f_2) = 0$  and so  $f_1 + f_2$  is injective by Axler 3.15.

Thus the set of all non-injective linear maps is not closed under addition and so cannot be a subspace of  $\mathcal{L}(V, W)$ .

12. The null space is the set of all vectors  $(v_1, v_2, v_3, v_4)$  with  $v_1 = 5v_2$  and  $v_3 = 7v_4$ .

I claim this space is spanned by the vectors  $5e_1 + e_2$  and  $7e_3 + e_4$ .

Suppose  $v = (5v_2, v_2, 7v_4, v_4)$  is any vector in the null space; obviously they all can be expressed this way.

Then  $v = v_2(5e_1 + e_2) + v_4(7e_3 + e_4)$ , and so  $v$  is a linear combination of the two basis vectors. Since  $v$  was an arbitrary vector in the null space, the null space is spanned by these two vectors.

Also, these two vectors are clearly linearly independent. If we have

$$a(5e_1 + e_2) + b(7e_3 + e_4) = 0$$

Then the left hand side is the vector  $(5a, a, 7b, b)$ . Since this vector equals zero, each component must be zero, and so in particular the second coordinate  $a$  and the fourth coordinate  $b$  must be zero. Thus the only linear combination of these vectors which gives zero is the one with all zero coefficients. Thus these two vectors are linearly independent.

Thus  $\dim \ker T$ , the cardinality of a basis for  $\ker T$ , is 2. By the rank-nullity theorem,

$$4 = \dim \mathbf{F}^4 = \dim \operatorname{im} T + \dim \ker T = \dim \operatorname{im} T + 2$$

So  $\dim \operatorname{im} T = 2$ . But the codomain of  $T$  is  $\mathbf{F}^2$ . Now note  $\operatorname{im} T$  is a subspace of  $\mathbf{F}^2$  and is spanned by two linearly independent vectors. Since  $\mathbf{F}^2$  has dimension 2, any two linearly independent vectors will span  $\mathbf{F}^2$  by Axler 2.38. Thus  $\operatorname{im} T = \mathbf{F}^2$  and so  $T$  is surjective.

19. Suppose  $T$  is injective and  $W$  is finite-dimensional. By Axler 3.22, the existence of this requires  $\dim V \leq \dim W$ .

Pick a basis  $\{v_i\}$  of  $V$ . Then  $\{T(v_i)\}$  is linearly independent in  $W$ . To prove this, choose a linear combination  $\sum a_i T(v_i)$  summing to zero.

Then

$$\sum a_i T(v_i) = T\left(\sum a_i v_i\right) = 0$$

But because  $T$  is injective, the only value mapping to 0 under the map  $T$  is zero. Thus  $\sum a_i v_i = 0$ , and since  $\{v_i\}$  is linearly independent, each  $a_i$  is zero. Thus we started with a linear combination of the vectors  $\{T(v_i)\}$  and showed that if this combination is zero, all the coefficients must be zero.

By Axler 2.32, since  $W$  is finite dimensional, the linearly independent set  $\{T(v_i)\}$  can be extended to a basis of  $W$ . Let this basis of  $W$  be composed of the vectors  $\{T(v_i)\}$  and some other vectors  $\{w_j\}$ . Define a map  $S : W \rightarrow V$  by:

$$S\left(\sum a_i T(v_i) + \sum b_j w_j\right) = \sum a_i v_i$$

This is well-defined because the representation of a vector as a combination of basis vectors is unique, and again the proof of Axler 3.4, with the right substitutions for the variables, shows linearity.

Now suppose a vector  $v$  is in  $V$ . Write  $v = \sum a_i v_i$ . Then

$$ST(v) = S\left(T\left(\sum a_i v_i\right)\right) = S\left(\sum a_i T(v_i)\right) = S\left(\sum a_i T(v_i) + \sum 0w_j\right) = \sum a_i v_i = v$$

and since  $v$  was arbitrary,  $ST$  is the identity on  $V$ . This proves one direction.

Now suppose  $T$  has a left inverse  $S$ . Then let  $u, v \in V$ , If  $Tu = Tv$  then  $STu = STv$  and, since  $ST$  is the identity, we conclude  $u = v$ . Since this holds for any pair of vectors  $u, v \in V$ , we see  $T$  is injective.

27. The rank nullity theorem makes this easy. I'll do it the hard way.

Firstly, we may decompose any vector  $v \in V$  as:

$$v = (v - Pv) + Pv$$

The first vector is in  $\ker P$  because

$$P(v - Pv) = Pv - P(Pv) = Pv - P^2v = Pv - Pv = 0$$

The second is clearly in  $\operatorname{im} P$ .

Thus  $V = \ker P + \operatorname{im} P$ .

This decomposition is also unique: suppose we have two decompositions of a vector  $v$ :

$$v = v_1 + Pv_2 = w_1 + Pw_2$$

where  $v_1, w_1 \in \ker P$  (clearly  $Pv_2, Pw_2 \in \operatorname{im} P$ ).

Then

$$Pv = P(v_1 + Pv_2) = Pv_1 + P^2v_2 = 0 + Pv_2 = Pv_2$$

But also, by the same logic

$$Pv = P(w_1 + Pw_2) = Pw_1 + P^2w_2 = 0 + Pw_2 = Pw_2$$

and so  $Pw_2 = Pv_2$ . Thus, by subtracting  $Pv_2 = Pw_2$  from both sides, we see  $v_1 = w_1$ . Thus the two decompositions are the same. Thus every vector  $v \in V$  decomposes uniquely into a sum of a vector in  $\ker P$  and a vector in  $\operatorname{im} P$ . Thus  $V = \ker P \oplus \operatorname{im} P$ .

29. To do this, we will first prove Problem 28: if a linear map  $D : P(\mathbf{F}) \rightarrow P(\mathbf{F})$  satisfies  $\deg Dp = \deg p - 1$  for all non-constant polynomials  $p$ , then  $D$  is surjective.

Proof: We show by induction that the set  $P_n(\mathbf{F})$  of polynomials with degree at most  $n$  is in the image of  $D$ . Since  $P(\mathbf{F}) = \bigcup_{n \in \mathbb{N}} P_n(\mathbf{F})$ , this will have shown that the whole  $P(\mathbf{F})$  is in  $\text{im } D$ , and thus  $D$  will have been shown to be surjective.

Firstly,  $P_0(\mathbf{F})$ , the set of the constants, is in the image. To see this, note that  $x$  has degree 1 and is not constant. So  $Dx$  has degree zero, thus is a constant (and a nonzero constant at that, by our definition of degree!).

So now pick any constant polynomial  $a$ , which is canonically identified with the *number*  $a$  in  $\mathbf{F}$ . Since  $\mathbf{F}$  is a field and  $Dx \neq 0$ , we can consider the multiplicative inverse  $(Dx)^{-1}$ .

Then  $D(a(Dx)^{-1}x) = a(Dx)^{-1} \cdot Dx$  by linearity, and so

$$D(a(Dx)^{-1}x) = a$$

Thus for an arbitrary constant polynomial  $a$ , we found a polynomial  $a(Dx)^{-1}x$  so that  $D$  sends  $a(Dx)^{-1}x$  to  $a$ .

Now suppose  $P_{n-1}(\mathbf{F}) \subset \text{im } D$ . Choose any polynomial  $r$  of degree  $n + 1$ .  $Dr$  has degree  $n$ . Write  $Dr = bx^n + s(x)$  where  $s$  has degree  $n - 1$ . Choose a polynomial  $\tilde{s}$  with  $D\tilde{s} = s$ ; we can do this by the induction assumption. Clearly  $\deg s = \deg \tilde{s} - 1$  and so  $\deg \tilde{s} = n < n + 1$ . Thus  $r - \tilde{s}$  has degree  $n$ . Furthermore,

$$D(r - \tilde{s}) = bx^n + s - D\tilde{s} = bx^n + s - s = bx^n$$

We know  $b \neq 0$  because otherwise  $\deg Dr < n$ , and we assumed  $\deg r = n + 1$  and so  $\deg Dr$  must be exactly  $n$ . Since  $\mathbf{F}$  is a field, we may consider the number  $b^{-1}$  and note that:

$$D(b^{-1}(r - \tilde{s})) = b^{-1}(bx^n) = (b^{-1}b)x^n = 1x^n = x^n$$

Let  $g = b^{-1}(r - \tilde{s})$ . Thus we have  $Dg = x^n$ .

Now let  $f = ax^n + p(x)$  with  $\deg p \leq n - 1$ . Clearly any polynomial of degree  $n$  can be written this way. Now since  $\deg p \leq n - 1$ , by the induction assumption  $p \in \text{im } D$ . Pick  $q \in P(\mathbf{F})$  so that  $Dq = p$ . Then note that:

$$D(ag + q) = aDg + Dq = ax^n + p = f$$

Thus we have shown that any polynomial  $f$  of degree  $n$  is in  $\text{im } D$ . Since any polynomial of degree  $\leq n - 1$  was assumed to be in  $\text{im } D$ , we conclude that if  $\deg f \leq n$  then  $f \in \text{im } D$ . Thus  $P_n(\mathbf{F}) \subset \text{im } D$ , as required.

By induction,  $P_n(\mathbf{F}) \subset \text{im } D$  for all  $n$ , and so  $\text{im } D$  contains all of  $P(\mathbf{F})$ .  $\text{im } D \subset P(\mathbf{F})$ , and so  $\text{im } D = P(\mathbf{F})$ . Thus  $D$  is surjective.

Now we prove Problem 29.

Firstly, the map  $E : q \mapsto 5q'' + 3q'$  is linear.

Proof:

$$\begin{aligned} E(aq + br) &= 5(aq + br)'' + 3(aq + br)' = 5(aq' + br')' + 3(aq' + br') \\ &= 5(aq'' + br'') + 3(aq' + br') = a(5q'') + b(5r'') + a(3q') + b(3r') \\ &= a(5q'' + 3q') + b(5r'' + 3r') \end{aligned}$$

$E$  also lowers the degree of non-constant polynomials by 1. This is because if  $q$  is not constant and has degree  $k$ , then  $q'$  has degree  $k - 1$ .  $q''$  will have degree at most  $k - 2$ —either  $k - 2$  exactly if  $q'$  is not constant, or  $-\infty$  (i.e.  $q'' = 0$ ) if  $q'$  is constant. In either case,  $3q'$  has degree  $k - 1$ , and  $5q''$  has degree at most  $k - 2$ , and so their sum will have degree  $k - 1$ .

Thus,  $E$  is surjective by Problem 28, and so for any  $p$  we can find a polynomial  $q$  so that  $E(q) = 5q'' + 3q' = p$ .